modified few things

src/Semantics.v
@@ -1,445 +1,265 @@
-Require Import Lib.CommonTactics Lib.FMap Lib.Struct.
-Require Export Syntax SemanticsExprAction. (* Should be "Require Export" *)
-Require Import String List.
+Require Import Bool List String Structures.Equalities FunctionalExtensionality Program.Equality Eqdep Eqdep_dec.
+Require Import Lib.Struct Lib.Word Lib.CommonTactics Lib.StringBound Lib.ilist Lib.FMap.
+Require Import Syntax.
+Require Export SemanticsExprAction.
 
 Set Implicit Arguments.
 
-Record LabelTP {A : Type} :=
-  { ruleMeth : option A
-  ; dms : CallsT
-  ; cms : CallsT
-  }.
+(*
+ * underscore to separate names only for lemmas and theorems
+ * Propositions start with upper case and no underscore
+ * Computable definitions start with lower case
+ *)
 
-Arguments LabelTP : clear implicits.
+Inductive UnitLabel :=
+| Rle: option string -> UnitLabel
+| Meth: option (Attribute (sigT SignT)) -> UnitLabel.
 
-Definition LabelT := LabelTP True.
-Definition RuleLabelT := LabelTP string.
+Record LabelT := { annot: option (option string);
+                   defs: MethsT;
+                   calls: MethsT }.
 
-Definition mapLabelTP {A B : Type} (f : A -> B) (l : LabelTP A)
-: LabelTP B :=
-  match l with
-    | Build_LabelTP rm dms cms => Build_LabelTP (option_map f rm) dms cms
+Section GivenModule.
+  Variable m: Modules.
+
+  Section GivenOldregs.
+    Variable o: RegsT.
+    Definition UpdatesT := RegsT.
+
+    Inductive Substep: UpdatesT -> UnitLabel -> MethsT -> Prop :=
+    | EmptyRule (HDomainEq: M.KeysEq o (map (@attrName _) (getRegInits m))):
+        Substep (M.empty _) (Rle None) (M.empty _)
+    | EmptyMeth (HDomainEq: M.KeysEq o (map (@attrName _) (getRegInits m))):
+        Substep (M.empty _) (Meth None) (M.empty _)
+    | SingleRule k (a: Action Void)
+                 (HInRules: List.In {| attrName := k; attrType := a |} (getRules m))
+                 (HOldRegs: M.KeysSubset o (map (@attrName _) (getRegInits m)))
+                 u cs (HAction: SemAction o (a type) u cs WO):
+        Substep u (Rle (Some k)) cs
+    | SingleMeth (f: DefMethT)
+                 (HIn: In f (getDefsBodies m))
+                 u cs argV retV
+                 (HOldRegs: M.KeysSubset o (map (@attrName _) (getRegInits m)))
+                 (HAction: SemAction o ((projT2 (attrType f)) type argV) u cs retV):
+        Substep u
+                (Meth (Some {| attrName := attrName f;
+                               attrType := (existT _ _ (argV, retV)) |})) cs.
+
+    Record SubstepRec :=
+      { upd: UpdatesT;
+        unitAnnot: UnitLabel;
+        cms: MethsT;
+        substep: Substep upd unitAnnot cms }.
+
+    Definition Substeps := list SubstepRec.
+
+    Definition canCombine (s1 s2: SubstepRec) :=
+      MF.Disj (upd s1) (upd s2) /\
+      (exists x, unitAnnot s1 = Meth x \/ unitAnnot s2 = Meth x) /\
+      MF.Disj (cms s1) (cms s2).
+
+    Inductive substepsComb: Substeps -> Prop :=
+    | NilSubsteps: substepsComb nil
+    | AddSubstep (s: SubstepRec) (ss: Substeps):
+        substepsComb ss -> (forall s', In s' ss -> canCombine s s') ->
+        substepsComb (s :: ss).
+
+    Fixpoint foldSSUpds (ss: Substeps) :=
+      match ss with
+        | x :: xs => MF.union (foldSSUpds xs) (upd x)
+        | nil => M.empty _
+      end.
+
+    Definition getSLabel (s: SubstepRec) :=
+      match s with
+        | {| unitAnnot := a; cms := cs |} =>
+          match a with
+            | Rle x => {| annot := Some x; defs := M.empty _; calls := cs |}
+            | Meth None => {| annot := None; defs := M.empty _; calls := cs |}
+            | Meth (Some {| attrName := n; attrType := t |}) =>
+              {| annot := None; defs := M.add n t (M.empty _); calls := cs |}
+          end
+      end.
+
+    Definition addLabelLeft' lnew lold :=
+      match lnew, lold with
+        | {| annot := a'; defs := d'; calls := c' |},
+          {| annot := a; defs := d; calls := c |} =>
+          {| annot := match a', a with
+                        | None, x => x
+                        | x, None => x
+                        | _, _ => None
+                      end; defs := MF.union d' d; calls := MF.union c' c |}
+      end.
+    
+    Definition addLabelLeft lold s := addLabelLeft' (getSLabel s) lold.
+
+    Fixpoint foldSSLabel (ss: Substeps) :=
+      match ss with
+        | x :: xs => addLabelLeft (foldSSLabel xs) x
+        | nil => {| annot := None; defs := M.empty _; calls := M.empty _ |}
+      end.
+
+(*
+    Definition getSSLabel (ss: Substeps) :=
+      fold_left addLabelLeft ss
+                {| annot := None; defs := M.empty _; calls := M.empty _ |}.
+*)
+
+    Lemma sigT_eq:
+      forall {A} (a: A) (B: A -> Type) (v1 v2: B a),
+        existT _ a v1 = existT _ a v2 ->
+        v1 = v2.
+    Proof. intros; inv H; apply Eqdep.EqdepTheory.inj_pair2 in H1; assumption. Qed.
+
+    Theorem signIsEq :
+      forall (l1 l2 : sigT SignT), {l1 = l2} + {l1 <> l2}.
+    Proof.
+      intros. destruct l1, l2.
+      destruct (SignatureT_dec x x0).
+      - induction e. destruct x, s, s0.
+        destruct (isEq arg t t1). induction e.
+        destruct (isEq ret t0 t2). induction e. left. reflexivity.
+        right. unfold not. intros. apply sigT_eq in H.
+        inversion H. apply n in H1. assumption.
+        right. unfold not. intros. apply sigT_eq in H.
+        inversion H. apply n in H1. assumption.
+      - right. unfold not. intros. inversion H. apply n in H1.
+        assumption.
+    Qed.
+
+    Definition hide (l: LabelT) :=
+      Build_LabelT (annot l) (MF.subtractKV signIsEq (defs l) (calls l))
+                   (MF.subtractKV signIsEq (calls l) (defs l)).
+
+    Definition wellHidden (l: LabelT) := M.KeysDisj (defs l) (getCalls m) /\
+                                         M.KeysDisj (calls l) (getDefs m).
+
+    Inductive Step: UpdatesT -> LabelT -> Prop :=
+      StepIntro ss (HSubsteps: substepsComb ss)
+                (HWellHidden: wellHidden (hide (foldSSLabel ss))) :
+        Step (foldSSUpds ss) (hide (foldSSLabel ss)).
+  End GivenOldregs. 
+
+  Inductive Multistep: RegsT -> UpdatesT -> list LabelT -> Prop :=
+  | NilMultistep o: Multistep o o nil
+  | Multi o a n (HMultistep: Multistep o n a)
+          u l (HStep: Step n u l):
+      Multistep o (MF.union u n) (l :: a).
+
+  Definition initRegs (init: list RegInitT): RegsT :=
+    makeMap (fullType type) evalConstFullT init.
+  Hint Unfold initRegs.
+
+  Definition LabelSeqT := list LabelT.
+
+  Inductive Behavior: UpdatesT -> LabelSeqT -> Prop :=
+  | BehaviorIntro a n (HMultistepBeh: Multistep (initRegs (getRegInits m)) n a):
+      Behavior n a.
+End GivenModule.
+
+Definition equivalentLabel p l1 l2 :=
+  p (defs l1) = defs l2 /\
+  p (calls l1) = calls l2 /\
+  match annot l1, annot l2 with
+    | Some _, Some _ => True
+    | None, None => True
+    | _, _ => False
   end.
 
-Definition NotBothRule (rm1 rm2 : option string) : Prop :=
-  rm1 = None \/ rm2 = None.
+Inductive equivalentLabelSeq p: LabelSeqT -> LabelSeqT -> Prop :=
+| NilEquivalentSeq: equivalentLabelSeq p nil nil
+| EquivalentSeq x xs y ys: equivalentLabel p x y -> equivalentLabelSeq p xs ys ->
+                           equivalentLabelSeq p (x :: xs) (y :: ys).
 
-Definition CanCombine (ul1 ul2: RegsT * RuleLabelT) : Prop :=
-  M.Disj (fst ul1) (fst ul2) /\
-  NotBothRule (ruleMeth (snd ul1)) (ruleMeth (snd ul2)) /\
-  M.Disj (dms (snd ul1)) (dms (snd ul2)) /\
-  M.Disj (cms (snd ul1)) (cms (snd ul2)).
+Definition traceRefines p m1 m2 :=
+  forall s1 sig1, Behavior m1 s1 sig1 ->
+                  exists s2 sig2, Behavior m2 s2 sig2 /\
+                                  equivalentLabelSeq p sig1 sig2.
 
-Definition mergeLabel {A : Type} (l1 l2 : LabelTP A) : LabelTP A := 
-  match l1, l2 with
-      Build_LabelTP rm1 ds1 cs1, Build_LabelTP rm2 ds2 cs2 =>
-      Build_LabelTP (match rm1 with | Some r => Some r | None => rm2 end) 
-                    (M.union ds1 ds2) 
-                    (M.union cs1 cs2)
-  end.
-
-Definition equivalent {A : Type} (l1 l2 : LabelTP A)
-           (p : LabelTP A -> LabelTP A) :=
-  l1 = p l2.
-
-Local Open Scope string.
-
-Inductive UnitStep : Modules -> RegsT -> RegsT -> RuleLabelT -> Type :=
-| EmptyStep :
-    forall (regInits : list RegInitT)
-           (rules : list (Attribute (Action Void)))
-           (meths : list DefMethT)
-           (oRegs : RegsT),
-      M.KeysSubset oRegs (namesOf regInits) ->
-      UnitStep (Mod regInits rules meths) oRegs (M.empty _)
-               (Build_LabelTP None (M.empty _) (M.empty _))
-| SingleRule : 
-  forall (ruleName : string) (ruleBody : Action (Bit 0))
-         (regInits : list RegInitT)
-         (rules : list (Attribute (Action Void)))
-         (meths : list DefMethT),
-    In (ruleName :: ruleBody)%struct rules ->
-    forall (oRegs news : RegsT) (calls : CallsT)
-           (retV : type (Bit 0)),
-      SemAction oRegs (ruleBody type) news calls retV ->
-      M.KeysSubset oRegs (namesOf regInits) ->
-      UnitStep (Mod regInits rules meths) oRegs news
-               (Build_LabelTP (Some ruleName) (M.empty _) calls)
-| SingleMeth :
-    forall (regInits : list RegInitT)
-           (rules : list (Attribute (Action Void)))
-           (meths : list DefMethT)
-           (oRegs : RegsT)
-           (calls : CallsT) (news : RegsT) 
-           (meth : DefMethT),
-      In meth meths ->
-      forall (argV : type (arg (objType (attrType meth))))
-             (retV : type (ret (objType (attrType meth))))
-             (udefs : CallsT),
-        SemAction oRegs (objVal (attrType meth) type argV) news calls retV ->
-        udefs = M.add meth {|
-                        objType := objType (attrType meth);
-                        objVal := (argV, retV) |} (M.empty _) ->
-        M.KeysSubset oRegs (namesOf regInits) ->
-        UnitStep (Mod regInits rules meths) oRegs news
-                 (Build_LabelTP None udefs calls)
-| LeftIntro :
-    forall (m1 m2 : Modules)
-           (oRegs1 oRegs2 oRegs news : RegsT)
-           (l : RuleLabelT),
-      M.KeysSubset oRegs2 (namesOf (getRegInits m2)) ->
-      UnitStep m1 oRegs1 news l ->
-      oRegs = M.union oRegs1 oRegs2 ->
-      UnitStep (ConcatMod m1 m2) oRegs news l
-| RightIntro :
-    forall (m1 m2 : Modules)
-           (oRegs1 oRegs2 oRegs news : RegsT)
-           (l : RuleLabelT),
-      M.KeysSubset oRegs1 (namesOf (getRegInits m1)) ->
-      UnitStep m2 oRegs2 news l ->
-      oRegs = M.union oRegs1 oRegs2 ->
-      UnitStep (ConcatMod m1 m2) oRegs news l.
-
-Inductive UnitSteps (m : Modules) (o : RegsT) : RegsT -> RuleLabelT -> Type :=
-| UnitSteps1 : forall {u l}, UnitStep m o u l -> UnitSteps m o u l
-| UnitStepsUnion : forall {u1 u2 : RegsT} {l1 l2 : RuleLabelT}, 
-                     UnitSteps m o u1 l1 -> UnitSteps m o u2 l2 
-                     -> CanCombine (u1, l1) (u2, l2)
-                     -> UnitSteps m o (M.union u1 u2) (mergeLabel l1 l2).
-
-Definition signIsEq :
-  forall (l1 l2 : Typed SignT), sumbool (l1 = l2) (l1 <> l2).
+Theorem staticDynCallsSubstep m o u rm cs:
+  Substep m o u rm cs ->
+  forall f, M.In f cs -> List.In f (getCalls m).
 Proof.
-  intros. destruct l1, l2. 
-  destruct (SignatureT_dec objType objType0).
-  - induction e. destruct objType, objVal, objVal0.
-    destruct (isEq arg t t1). induction e.
-    destruct (isEq ret t0 t2). induction e. left. reflexivity.
-    right. unfold not. intros. apply typed_eq in H.
-    inversion H. apply n in H1. assumption.
-    right. unfold not. intros. apply typed_eq in H.
-    inversion H. apply n in H1. assumption.
-  - right. unfold not. intros. inversion H. apply n in H1.
-    assumption.
+  admit.
 Qed.
 
-Definition hide {A : Type} (l : LabelTP A) : LabelTP A :=
-  match l with
-      Build_LabelTP rm ds cs => 
-      Build_LabelTP rm (M.subtractKV signIsEq ds cs)
-                    (M.subtractKV signIsEq cs ds)
-  end.
+Theorem staticDynDefsSubstep m o u far cs:
+  Substep m o u (Meth (Some far)) cs ->
+  List.In (attrName far) (getDefs m).
+Proof.
+  intros.
+  dependent induction H; simpl in *.
+  unfold getDefs in *.
+  clear - HIn.
+  induction (getDefsBodies m).
+  - intuition.
+  - simpl in *.
+    destruct HIn.
+    + subst.
+      left; intuition.
+    + right; intuition.
+Qed.
 
-Definition wellHidden {A : Type} (l : LabelTP A) (m : Modules) :=
-  match l with
-      Build_LabelTP rm ds cs =>
-      M.KeysDisj ds (getCmsMod m)
-      /\ M.KeysDisj cs (getDmsMod m)
-  end.
+Theorem staticDynCallsSubsteps m o ss:
+  forall f, M.In f (calls (foldSSLabel (m := m) (o := o) ss)) -> In f (getCalls m).
+Proof.
+  intros.
+  induction ss; simpl in *.
+  - exfalso.
+    apply (proj1 (MF.F.P.F.empty_in_iff _ _) H).
+  - unfold addLabelLeft, addLabelLeft' in *.
+    destruct a.
+    simpl in *.
+    destruct unitAnnot0.
+    + destruct (foldSSLabel ss); simpl in *.
+      pose proof (MF.union_In _ H) as sth.
+      destruct sth.
+      * apply (staticDynCallsSubstep substep0); intuition.
+      * intuition.
+    + destruct (foldSSLabel ss); simpl in *.
+      dependent destruction o0; simpl in *.
+      * dependent destruction a; simpl in *.
+        pose proof (MF.union_In _ H) as sth.
+        { destruct sth.
+          - apply (staticDynCallsSubstep substep0); intuition.
+          - intuition.
+        }
+      * pose proof (MF.union_In _ H) as sth.
+        { destruct sth.
+          - apply (staticDynCallsSubstep substep0); intuition.
+          - intuition.
+        }
+Qed.
 
-Inductive Step (m : Modules) (o u : RegsT) : RuleLabelT -> Type :=
-  MkStep : forall {l l': RuleLabelT},
-             UnitSteps m o u l ->
-             l' = hide l -> wellHidden l' m ->
-             Step m o u l'.
+Theorem staticDynDefsSubsteps m o ss:
+  forall f, M.In f (defs (foldSSLabel (m := m) (o := o) ss)) -> In f (getDefs m).
+Proof.
+  intros.
+  induction ss; simpl in *.
+  - exfalso.
+    apply (proj1 (MF.F.P.F.empty_in_iff _ _) H).
+  - unfold addLabelLeft, addLabelLeft' in *.
+    destruct a.
+    simpl in *.
+    destruct unitAnnot0.
+    + destruct (foldSSLabel ss); simpl in *.
+      rewrite MF.union_empty_L in H.
+      intuition.
+    + destruct (foldSSLabel ss); simpl in *.
+      dependent destruction o0; simpl in *.
+      * dependent destruction a; simpl in *.
+        pose proof (MF.union_In _ H) as sth.
+        { destruct sth.
+          - apply MF.F.P.F.add_in_iff in H0.
+            destruct H0.
+            + subst.
+              apply (staticDynDefsSubstep substep0).
+            + exfalso; apply ((proj1 (MF.F.P.F.empty_in_iff _ _)) H0).
+          - intuition.
+        }
+      * rewrite MF.union_empty_L in H.
+        intuition.
+Qed.
 
-Inductive MultiStep (m : Modules) (regs : RegsT) : RegsT -> list RuleLabelT -> Prop :=
-| MSNil : MultiStep m regs regs nil
-| MSMulti :
-    forall regs' labels,
-      MultiStep m regs regs' labels ->
-      forall l u,
-        Step m regs' u l ->
-        forall (regs'' : RegsT),
-          regs'' = M.update regs' u ->
-          MultiStep m regs regs'' (l :: labels).
-
-Section MakeMap.
-  Variable A: Type.
-  Variable f1 f2: A -> Type.
-  Variable f: forall x, f1 x -> f2 x.
-
-  Fixpoint makeMap (l: list (Attribute (Typed f1))) : M.t (Typed f2) :=
-    match l with
-      | nil => M.empty _
-      | {| attrName := n; attrType := {| objVal := rv |} |} :: xs =>
-        M.add n {| objVal := f rv |} (makeMap xs)
-    end.  
-End MakeMap.
-
-Definition initRegs (init: list RegInitT): RegsT := makeMap (fullType type) evalConstFullT init.
-Hint Unfold initRegs.
-
-Inductive Behavior (m : Modules) : RegsT -> list LabelT -> Prop :=
-  MkBehavior :
-    forall newRegs labels labels',
-      MultiStep m (initRegs (getRegInits m)) newRegs labels ->
-      labels' = (List.map (mapLabelTP (fun _ => I)) labels) ->
-      Behavior m newRegs labels'.
-
-Definition TraceRefines (mimpl mspec : Modules) (f : LabelT -> LabelT) :=
-  forall simp limp,        Behavior mimpl simp         limp ->
-  exists (sspec : RegsT),  Behavior mspec sspec (map f limp).
-
-Section Decomposition.
-  Variable rulesImp rulesSpec: list string.
-  Variable dmsImp dmsSpec: list DefMethT.
-  Variable imp spec: Modules.
-  Variable stateMap: RegsT -> RegsT.
-  Variable ruleMap: string -> string.
-  Variable p : (CallsT * CallsT) -> (CallsT * CallsT).
-
-  Definition pMod {A : Type} (f : A -> A) (l : LabelTP A) : LabelTP A
-    := match l with
-    | Build_LabelTP rm dm cm => let (dm', cm') := p (dm, cm) in
-       Build_LabelTP (option_map f rm) dm' cm'
-    end.
-
-  Definition pRL := pMod ruleMap.
-
-  Hypothesis pmerge : forall (ds1 ds2 cs1 cs2 : CallsT) (rm1 rm2 : option string)
-    , let l1 := Build_LabelTP rm1 ds1 cs1 in 
-      let l2 := Build_LabelTP rm2 ds2 cs2 in
-       M.Disj ds1 ds2 -> M.Disj cs1 cs2
-     -> NotBothRule rm1 rm2
-     -> mergeLabel (pRL l1) (pRL l2) = pRL (mergeLabel l1 l2).
-
-  Hypothesis phide : forall (l : RuleLabelT), pRL (hide l) = hide (pRL l).
-
-  Hypothesis pwellHidden : forall (l : RuleLabelT), 
-   wellHidden (hide l) imp -> wellHidden (pRL (hide l)) spec.
-
-  Variable T : forall {oImp nImp lImp}, UnitStep imp oImp nImp lImp 
-             -> (RegsT * RuleLabelT).
-
-  Fixpoint Ts {oImp nImp lImp} (steps : UnitSteps imp oImp nImp lImp)
-      : RegsT * RuleLabelT
-      := match steps with
-    | UnitSteps1 _ _ step => T step
-    | UnitStepsUnion _ _ _ _ step1 step2 canCombine => 
-      let (u1, l1) := Ts step1 in
-      let (u2, l2) := Ts step2 in
-      (M.union u1 u2, mergeLabel l1 l2)
-    end.
-
-  Let Ts' {oImp nImp lImp} (step : Step imp oImp nImp lImp)
-      : RegsT * RuleLabelT
-      := match step with
-    | MkStep _ _ steps _ _  => Ts steps
-    end.
-
-  Hypothesis stateMapBeginsWell :
-    stateMap (initRegs (getRegInits imp)) = initRegs (getRegInits spec).
-
-  Hypothesis stateMapModular : forall (oImp u1 u2 uSpec1 uSpec2 : RegsT),
-    M.Disj u1 u2 -> M.Disj uSpec1 uSpec2
-  -> M.update (stateMap oImp) uSpec1 = stateMap (M.update oImp u1)
-  -> M.update (stateMap oImp) uSpec2 = stateMap (M.update oImp u2)
-  -> M.update (stateMap oImp) (M.union uSpec1 uSpec2) 
-  = stateMap (M.update oImp (M.union u1 u2)).
-
-  Hypothesis consistentSubstepMap : forall {oImp lImp nImp}
-   , (exists ruleLabel, Behavior imp oImp ruleLabel)
-   -> forall (step : UnitStep imp oImp nImp lImp)
-   , match T step with (nSpec, lSpec) =>
-      let oSpec := stateMap oImp in
-        (M.update oSpec nSpec = stateMap (M.update oImp nImp)
-      /\ equivalent lSpec lImp pRL)
-      * UnitStep spec oSpec nSpec lSpec
-     end.
-
-  Hypothesis specShouldCombine : forall {oImp} 
-  , (exists ruleLabel, Behavior imp oImp ruleLabel)
-  -> forall {nImp1 lImp1} (step1 : UnitStep imp oImp nImp1 lImp1)
-      {nImp2 lImp2} (step2 : UnitStep imp oImp nImp2 lImp2)
-  , CanCombine (nImp1, lImp1) (nImp2, lImp2)
-  -> CanCombine (T step1) (T step2).
-
-  Lemma pBeforeAfter : forall (l : RuleLabelT),
-    pMod id (mapLabelTP (fun _ : string => I) l) =
-     mapLabelTP (fun _ : string => I) (pRL l).
-  Proof. intros. unfold pRL, pMod.
-  destruct l. simpl.
-  destruct (p (dms0, cms0)). simpl.
-  destruct ruleMeth0; simpl; unfold id; reflexivity.
-  Qed.
-
-  Lemma canCombineLeft :
-    forall {t u1 u2 l1 l2},
-      CanCombine t (M.union u1 u2, mergeLabel l1 l2) ->
-      CanCombine t (u1, l1).
-  Proof. 
-    intros.
-    destruct l1 as [rm1 ds1 cs1].
-    destruct l2 as [rm2 ds2 cs2].
-    unfold CanCombine in H; dest; simpl in *.
-    constructor; try (eapply M.Disj_union_1; eassumption).
-    unfold NotBothRule in *.
-    destruct rm1.
-    - simpl; destruct H0; [|discriminate].
-      repeat split.
-      + left; auto.
-      + eapply M.Disj_union_1; eauto.
-      + eapply M.Disj_union_1; eauto.
-    - repeat split.
-      + right; auto.
-      + eapply M.Disj_union_1; eauto.
-      + eapply M.Disj_union_1; eauto.
-  Qed.
-
-  Lemma canCombineRight :
-    forall {t u1 u2 l1 l2},
-      CanCombine t (M.union u1 u2, mergeLabel l1 l2) ->
-      CanCombine t (u2, l2).
-  Proof.
-    intros.
-    destruct l1 as [rm1 ds1 cs1].
-    destruct l2 as [rm2 ds2 cs2].
-    unfold CanCombine in H; dest; simpl in *.
-    constructor; try (eapply M.Disj_union_2; eassumption).
-    unfold NotBothRule in *.
-    destruct rm1.
-    - simpl; destruct H0; [|discriminate].
-      repeat split.
-      + left; auto.
-      + eapply M.Disj_union_2; eauto.
-      + eapply M.Disj_union_2; eauto.
-    - simpl; destruct H0.
-      + repeat split.
-        * left; auto.
-        * eapply M.Disj_union_2; eauto.
-        * eapply M.Disj_union_2; eauto.
-      + repeat split.
-        * right; auto.
-        * eapply M.Disj_union_2; eauto.
-        * eapply M.Disj_union_2; eauto.
-  Qed.
-
-  Lemma canCombineMerge : forall {t u1 u2 l1 l2},
-    CanCombine t (u1, l1)
-  -> CanCombine t (u2, l2)
-  -> CanCombine t (M.union u1 u2, mergeLabel l1 l2).
-  Proof.
-    admit.
-    (* intros. destruct t as [uL [rmL csL dsL]].  *)
-    (* destruct (mergeLabel l1 l2) as [rm1 cs ds] eqn:labeleqn. *)
-    (* inversion H; inversion H0; inversion labeleqn; subst. *)
-    (* econstructor. apply M.Disj_union; assumption. *)
-    (* apply M.Disj_union; assumption. *)
-    (* apply M.Disj_union; assumption. *)
-    (* unfold NotBothRule in *; destruct rmL, rm2, rm4; intuition. *)
-  Qed.  
-
-  Lemma canCombineSym : forall {t1 t2},
-    CanCombine t1 t2 -> CanCombine t2 t1.
-  Proof.
-    admit.
-   (* intros t1 t2 H; *)
-   (* inversion H; clear H; subst;  *)
-   (* constructor; eauto using M.Disj_comm. *)
-   (* unfold NotBothRule in *. *)
-   (* destruct rm1, rm2; intuition. *)
-  Qed. 
-
-  Lemma specShouldCombines : forall {oImp} 
-  , (exists ruleLabel, Behavior imp oImp ruleLabel)
-  -> forall {nImp1 lImp1} (step1 : UnitSteps imp oImp nImp1 lImp1)
-      {nImp2 lImp2} (step2 : UnitSteps imp oImp nImp2 lImp2)
-  , CanCombine (nImp1, lImp1) (nImp2, lImp2)
-  -> CanCombine (Ts step1) (Ts step2).
-  Proof. 
-    intros oImp H nImp1 lImp1 US1. induction US1.
-    - intros nImp2 lImp2 US2. induction US2.
-      + apply specShouldCombine; assumption.
-      + intros.
-        simpl in IHUS2_1, IHUS2_2.
-        pose proof (IHUS2_1 (canCombineLeft H0)) as H21.
-        pose proof (IHUS2_2 (canCombineRight H0)) as H22.
-        simpl. destruct (Ts US2_1). destruct (Ts US2_2).
-        apply canCombineMerge; assumption.
-    - simpl in *. intros. apply canCombineSym.
-      destruct (Ts US1_1). destruct (Ts US1_2).
-      apply canCombineMerge; apply canCombineSym;
-      [apply IHUS1_1 | apply IHUS1_2]; try assumption;
-      apply canCombineSym in H0;
-      apply canCombineSym. 
-      eapply canCombineLeft; eassumption.
-      eapply canCombineRight; eassumption.    
-  Qed.
-  
-Require CommonTactics.
-
-  Lemma consistentUnitStepsMap : forall oImp lImp nImp
-    , (exists ruleLabel, Behavior imp oImp ruleLabel)
-      -> forall (steps : UnitSteps imp oImp nImp lImp)
-      , let (nSpec, lSpec) := Ts steps in
-        let oSpec := stateMap oImp in
-        (M.update oSpec nSpec = stateMap (M.update oImp nImp)
-         /\ equivalent lSpec lImp pRL)
-        * UnitSteps spec oSpec nSpec lSpec.
-  Proof.
-    admit.
-  (*   intros. *)
-  (*   induction steps; intros. *)
-  (*   - pose proof (consistentSubstepMap H u0). simpl in *. *)
-  (*     destruct (T u0) as [uSpec lSpec]. *)
-  (*     intuition. constructor. assumption. *)
-  (* - pose proof (specShouldCombines H steps1 steps2 c). *)
-  (*   simpl in *. *)
-  (*   destruct (Ts steps1) as [uSpec1 lSpec1]. *)
-  (*   destruct (Ts steps2) as [uSpec2 lSpec2]. *)
-  (*   intuition.  *)
-  (*   CommonTactics.inv c. CommonTactics.inv H0. *)
-  (*   apply stateMapModular; assumption. *)
-  (*   unfold equivalent in *. subst. *)
-  (*   CommonTactics.inv c. *)
-  (*   apply pmerge; assumption. *)
-  (*   apply UnitStepsUnion. assumption. assumption. *)
-  (*   unfold equivalent in *. *)
-  (*   assumption. *)
-  Qed.
-  
-  Lemma consistentStepMap : forall oImp lImp nImp
-    , (exists ruleLabel, Behavior imp oImp ruleLabel)
-      -> forall (step : Step imp oImp nImp lImp)
-      , let (nSpec, lSpec) := Ts' step in
-        let oSpec := stateMap oImp in
-        (M.update oSpec nSpec = stateMap (M.update oImp nImp))
-        * Step spec oSpec nSpec (pRL lImp).
-  Proof. 
-    intros.
-    destruct step eqn:stepeqn.
-    pose proof (consistentUnitStepsMap H u). simpl in *.
-    destruct (Ts u) as [nSpec lSpec]. 
-    intuition.  
-    econstructor. eassumption.
-    unfold equivalent in *. rewrite e.
-    rewrite H1. apply phide.
-    unfold equivalent in *. subst.
-    apply (pwellHidden _ w).
-  Qed. 
-
-  Theorem decomposition : TraceRefines imp spec (pMod id).
-  Proof.
-    unfold TraceRefines. intros.
-    exists (stateMap simp).
-    pose proof H.
-    inversion H0; clear H0; subst.
-    econstructor.
-    Focus 2. instantiate (1 := map pRL labels).
-    repeat rewrite map_map. apply map_ext.
-    intros. apply pBeforeAfter.
-    induction H1.
-    - rewrite <- stateMapBeginsWell. apply MSNil.
-    - assert (Behavior imp regs' (map (mapLabelTP (fun _ : string => I)) labels)).
-      econstructor. eassumption. reflexivity.
-      pose proof (consistentStepMap (ex_intro _ _ H2) X).
-      destruct (Ts' X) eqn:Ts'X.
-      destruct X0 as [HT1 HT2].
-      apply MSMulti with (regs' := stateMap regs') (u := r).
-      apply IHMultiStep. assumption.
-      assumption.
-      rewrite H0. rewrite <- HT1. reflexivity.
-  Qed.
-
-End Decomposition.
+Definition reachable m o := exists sig, Behavior m o sig.
