src/Decomposition.v
@@ -1,0 +1,426 @@
+Require Import Bool List String Structures.Equalities FunctionalExtensionality Program.Equality Eqdep Eqdep_dec.
+Require Import Lib.Struct Lib.Word Lib.CommonTactics Lib.StringBound Lib.ilist Lib.FMap.
+Require Import Syntax Semantics.
+
+Set Implicit Arguments.
+
+Definition DomainSubset A B (s1: M.t A) (s2: M.t B) := forall k, M.In k s1 -> M.In k s2.
+
+Section MapSet.
+  Variable A: Type.
+  Variable p: M.key -> A -> option A.
+
+  Definition rmModify k v m := match p k v with
+                                 | None => m
+                                 | Some v' => M.add k v' m
+                               end.
+  Definition mapSet s :=
+    Map.fold rmModify s (M.empty _).
+
+  Theorem mapSetEmpty: mapSet (M.empty _) = M.empty _.
+  Proof.
+    unfold mapSet, M.fold; reflexivity.
+  Qed.
+
+  Lemma mapSetSubset s: DomainSubset (mapSet s) s.
+  Proof.
+    apply (MF.map_induction (P := fun s => DomainSubset (mapSet s) s)); unfold DomainSubset; intros.
+    - rewrite mapSetEmpty in *.
+      intuition.
+    - unfold mapSet in H1.
+      rewrite MF.P.fold_add in H1; fold (mapSet m) in *; intuition.
+      + apply MF.P.F.add_in_iff.
+        unfold rmModify in *.
+        destruct (p k v).
+        apply MF.P.F.add_in_iff in H1.
+        destruct H1; intuition.
+        right; apply (H _ H1).
+      + clear; unfold Morphisms.Proper, Morphisms.respectful; intros; subst.
+        apply M.leibniz in H1; subst.
+        intuition.
+      + clear; unfold MF.P.transpose_neqkey; intros.
+        unfold rmModify.
+        destruct (p k e), (p k' e');
+          try apply MF.transpose_neqkey_Equal_add; intuition.
+  Qed.
+        
+  Theorem mapSetAddOne k v:
+    mapSet (M.add k v (M.empty _)) =
+    match p k v with
+      | Some argRet => M.add k argRet (M.empty _)
+      | None => M.empty _
+    end.
+  Proof.
+    case_eq (p k v); unfold mapSet, rmModify, M.fold; simpl.
+    intros a H.
+    rewrite H; reflexivity.
+    intros H.
+    rewrite H; reflexivity.
+  Qed.
+End MapSet.
+
+(*
+Definition transformLabel l p :=
+  match l with
+    | {| annot := a; defs := dfs; calls := clls |} => {| annotStrip := match a with
+                                                                         | Some _ => true
+                                                                         | None => false
+                                                                       end;
+                                                         defsStrip := p dfs;
+                                                         callsStrip := p clls |}
+  end.
+
+Definition equivalentLabel p l1 l2 :=
+  transformLabel l1 p = transformLabel l2 (fun x => x).
+*)
+
+
+Section Decomposition.
+  Variable imp spec: Modules.
+  Variable theta: RegsT -> RegsT.
+  Variable ruleMap: RegsT -> string -> option string.
+  Variable p: string -> (sigT SignT) -> option (sigT SignT).
+  Variable thetaInit: theta (initRegs (getRegInits imp)) = initRegs (getRegInits spec).
+  Variable thetaGood: forall o, M.KeysEq (theta o) (map (@attrName _)
+                                                         (getRegInits spec)).
+  Variable defSubset: forall f, In f (getDefs spec) -> In f (getDefs imp).
+  Variable callSubset: forall f, In f (getCalls spec) -> In f (getCalls imp).
+
+  Variable substepRuleMap:
+    forall oImp uImp rule csImp,
+      Substep imp oImp uImp (Rle (Some rule)) csImp ->
+      { uSpec |
+        Substep spec (theta oImp) uSpec (Rle (ruleMap oImp rule)) (mapSet p csImp) /\
+        forall o, MF.union uSpec (theta o) = theta (MF.union uImp o) }.
+
+  Definition liftP meth :=
+    match meth with
+      | (n :: t)%struct => match p n t with
+                             | None => None
+                             | Some v => Some (n :: v)%struct
+                           end
+    end.
+
+  Variable substepMethMap:
+    forall oImp uImp meth csImp,
+      Substep imp oImp uImp (Meth (Some meth)) csImp ->
+      { uSpec |
+        Substep spec (theta oImp) uSpec (Meth (liftP meth)) (mapSet p csImp) /\
+        forall o, MF.union uSpec (theta o) = theta (MF.union uImp o) }.
+
+  Definition ruleMapEmpty o u cs (s: Substep imp o u (Rle None) cs):
+    { uSpec |
+      Substep spec (theta o) uSpec (Rle None) (mapSet p cs) /\
+      forall o', MF.union uSpec (theta o') = theta (MF.union u o') }.
+  Proof.
+    refine (exist _ (M.empty _) _);
+    abstract (
+        inversion s; subst; rewrite mapSetEmpty;
+        constructor;
+        [ constructor; apply thetaGood |
+          repeat rewrite MF.union_empty_L; intuition]).
+  Defined.
+
+  Definition methMapEmpty o u cs (s: Substep imp o u (Meth None) cs):
+    { uSpec |
+      Substep spec (theta o) uSpec (Meth None) (mapSet p cs) /\
+      forall o', MF.union uSpec (theta o') = theta (MF.union u o') }.
+  Proof.
+    refine (exist _ (M.empty _) _);
+    abstract (
+        inversion s; subst; rewrite mapSetEmpty;
+        constructor;
+        [ constructor; apply thetaGood |
+          repeat rewrite MF.union_empty_L; intuition]).
+  Defined.
+
+  Definition xformUnitAnnot o rm :=
+    match rm with
+      | Rle (Some rule) => Rle (ruleMap o rule)
+      | Meth (Some meth) => Meth (liftP meth)
+      | Rle None => Rle None
+      | Meth None => Meth None
+    end.
+
+  Definition substepMap o u rm cs (s: Substep imp o u rm cs) :=
+    match rm return Substep imp o u rm cs ->
+                    { uSpec |
+                      Substep spec (theta o) uSpec (xformUnitAnnot o rm) (mapSet p cs) /\
+                      forall o', MF.union uSpec (theta o') = theta (MF.union u o') } with
+      | Rle (Some rule) => fun s => substepRuleMap s
+      | Meth (Some meth) => fun s => substepMethMap s
+      | Rle None => fun s => ruleMapEmpty s
+      | Meth None => fun s => methMapEmpty s
+    end s.
+
+  Definition xformSubstepRec o (s': SubstepRec imp o) :=
+    match s' with
+      | {| upd := u; unitAnnot := rm; cms := cs; substep := s |} =>
+        match substepMap s with
+          | exist uSpec (conj sSpec _) =>
+            {| upd := uSpec; unitAnnot := xformUnitAnnot o rm;
+               cms := mapSet p cs; substep := sSpec |}
+        end
+    end.
+
+  Variable specCanCombine:
+    forall o (s1 s2: SubstepRec imp o),
+      canCombine s1 s2 -> canCombine (xformSubstepRec s1) (xformSubstepRec s2).
+
+  Theorem substepsSpecComb o:
+    forall (ss: Substeps imp o), substepsComb ss ->
+                                 substepsComb (map (@xformSubstepRec o) ss).
+  Proof.
+    induction ss; intros; simpl in *; constructor; intros.
+    - dependent destruction H; intuition.
+    - dependent destruction H.
+      pose proof (proj1 (in_map_iff (@xformSubstepRec o) ss s') H1) as [sImp [eqS inS]].
+      specialize (H0 _ inS); subst.
+      apply specCanCombine; intuition.
+  Qed.
+
+  Definition xformLabel o l :=
+    match l with
+      | {| annot := a; defs := dfs; calls := clls |} =>
+        {| annot := match a with
+                      | Some (Some r) => Some (ruleMap o r)
+                      | Some None => Some None
+                      | None => None
+                    end;
+           defs := mapSet p dfs;
+           calls := mapSet p clls |}
+    end.
+
+  Lemma wellHiddenSpec o l:
+    wellHidden imp l ->
+    wellHidden spec (xformLabel o l).
+  Proof.
+    intros [dHid cHid].
+    unfold wellHidden in *.
+    unfold xformLabel; destruct l; simpl in *.
+    clear - defSubset callSubset dHid cHid.
+    pose proof (mapSetSubset p defs) as dH.
+    pose proof (mapSetSubset p calls) as cH.
+    unfold DomainSubset, M.KeysDisj in *.
+    constructor; intros.
+    - specialize (dH _ H).
+      specialize (callSubset _ H0).
+      specialize (dHid _ dH).
+      intuition.
+    - specialize (cH _ H).
+      specialize (defSubset _ H0).
+      specialize (cHid _ cH).
+      intuition.
+  Qed.
+
+  Lemma subtractKVMapSet l1:
+    forall l2,
+      (forall x v1 v2, M.MapsTo x v1 l1 -> M.MapsTo x v2 l2 -> v1 = v2) ->
+      mapSet p (MF.subtractKV signIsEq l1 l2) = MF.subtractKV signIsEq (mapSet p l1)
+                                                              (mapSet p l2).
+  Proof.
+    apply (MF.map_induction
+             (P := fun l1 => forall l2 : M.t (sigT SignT),
+                       (forall (x : M.key) (v1 v2 : sigT SignT), M.MapsTo x v1 l1 ->
+                                                                 M.MapsTo x v2 l2 -> v1 = v2) ->
+                       mapSet p (MF.subtractKV signIsEq l1 l2) =
+                       MF.subtractKV signIsEq (mapSet p l1) (mapSet p l2))); intros; simpl in *.
+    - rewrite (MF.subtractKV_empty_1).
+      rewrite mapSetEmpty.
+      rewrite (MF.subtractKV_empty_1).
+      reflexivity.
+    - admit.
+  Qed.
+
+  Lemma subtractKVDefn k l1 l2 v1 v2:
+    M.MapsTo k v1 l1 -> M.MapsTo k v2 l2 -> v1 <> v2 ->
+    M.In k (MF.subtractKV signIsEq l1 l2).
+  Proof.
+    admit.
+  Qed.
+  
+  Theorem wellHiddenEq1 m l:
+    M.KeysSubset (defs l) (getDefs m) ->
+    M.KeysSubset (calls l) (getCalls m) ->
+    wellHidden m (hide l) ->
+    forall x v1 v2, M.MapsTo x v1 (defs l) ->
+                    M.MapsTo x v2 (calls l) ->
+                    v1 = v2.
+  Proof.
+    intros; unfold M.KeysSubset, wellHidden, M.KeysDisj in *.
+    destruct l; unfold hide; simpl in *.
+    destruct H1 as [d c].
+    destruct (signIsEq v1 v2).
+    - assumption.
+    - pose proof (subtractKVDefn H2 H3 n) as sthSub.
+      assert (sthIn: M.In x calls) by
+          (unfold M.In, M.Raw.PX.In, M.MapsTo in *; exists v2; assumption).
+      specialize (H0 _ sthIn).
+      exfalso; apply (d _ sthSub H0).
+  Qed.
+    
+  Theorem xformLabelHideCommute o l:
+    (forall x v1 v2, M.MapsTo x v1 (defs l) -> M.MapsTo x v2 (calls l) -> v1 = v2) ->
+    xformLabel o (hide l) = hide (xformLabel o l).
+  Proof.
+    intros Hyp.
+    unfold xformLabel, hide.
+    destruct l.
+    assert (Hyp2: forall x v1 v2, M.MapsTo x v1 calls -> M.MapsTo x v2 defs -> v1 = v2) by
+        (intros ? ? ? M1 M2; apply eq_sym; apply (Hyp x v2 v1); intuition).
+    destruct annot; simpl in *.
+    - destruct o0; simpl in *; f_equal; rewrite subtractKVMapSet; intuition.
+    - f_equal; rewrite subtractKVMapSet; intuition.
+  Qed.
+
+  Theorem mapSetUnionCommute l1 l2:
+    mapSet p (MF.union l1 l2) = MF.union (mapSet p l1) (mapSet p l2).
+  Proof.
+    admit.
+  Qed.      
+  
+  Theorem xformLabelAddLabelCommute l1 l2:
+    forall o,
+      xformLabel o (addLabelLeft' l1 l2) = addLabelLeft' (xformLabel o l1) (xformLabel o l2).
+  Proof.
+    intros.
+    unfold addLabelLeft', xformLabel; simpl in *.
+    destruct l1, l2; simpl in *.
+    destruct annot, annot0;
+      repeat (try destruct o0; try destruct o1; simpl in *;
+              repeat rewrite mapSetUnionCommute; intuition).
+  Qed.
+
+  Lemma xformLabelGetSLabelCommute o a:
+    xformLabel o (getSLabel (o := o) a) = getSLabel (xformSubstepRec a).
+  Proof.
+    destruct a; simpl in *.
+    destruct (substepMap substep).
+    destruct a.
+    simpl.
+    unfold xformLabel, xformUnitAnnot.
+    destruct unitAnnot; destruct o0; try rewrite mapSetEmpty; intuition.
+    destruct a.
+    unfold liftP.
+    rewrite mapSetAddOne.
+    destruct (p attrName attrType); intuition.
+  Qed.
+    
+  Theorem xformLabelFoldCommute o ss:
+    xformLabel o (foldSSLabel (o := o) ss) = foldSSLabel (map (@xformSubstepRec _) ss).
+  Proof.
+    induction ss; simpl in *; try rewrite mapSetEmpty.
+    - reflexivity.
+    - unfold addLabelLeft in *.
+      rewrite xformLabelAddLabelCommute.
+      f_equal; intuition.
+      apply xformLabelGetSLabelCommute.
+  Qed.    
+  
+  Theorem xformLabelHide o:
+    forall(ss: Substeps imp o) (ssGd: wellHidden imp (hide (foldSSLabel ss))),
+      hide (foldSSLabel (map (@xformSubstepRec _) ss)) =
+      xformLabel o (hide (foldSSLabel ss)).
+  Proof.
+    intros.
+    rewrite xformLabelHideCommute.
+    f_equal.
+    apply eq_sym; apply xformLabelFoldCommute.
+    apply (wellHiddenEq1 (m := imp)).
+    - unfold M.KeysSubset; apply (staticDynDefsSubsteps ss).
+    - unfold M.KeysSubset; apply (staticDynCallsSubsteps ss).
+    - intuition.
+  Qed.
+
+  Lemma unionCommute' o a state:
+    MF.union (upd (xformSubstepRec (o := o) a)) (theta state) = theta (MF.union (upd a) state).
+  Proof.
+    destruct a; simpl in *.
+    destruct (substepMap substep).
+    destruct a; simpl in *.
+    intuition.
+  Qed.
+
+  Lemma unionCommute o ss:
+    forall state,
+      MF.union (foldSSUpds (map (xformSubstepRec (o:=o)) ss)) (theta state) =
+      theta (MF.union (foldSSUpds ss) state).
+  Proof.
+    induction ss; intros; simpl in *.
+    - repeat rewrite MF.union_empty_L; reflexivity.
+    - rewrite <- MF.union_assoc.
+      rewrite <- MF.union_assoc.
+      rewrite unionCommute'.
+      apply (IHss (MF.union (upd a) state)).
+  Qed.
+
+  Theorem stepMap o u l (s: Step imp o u l):
+    exists uSpec,
+      Step spec (theta o) uSpec (xformLabel o l) /\
+      MF.union uSpec (theta o) = theta (MF.union u o).
+  Proof.
+    destruct s as [ss ssGd].
+    exists (foldSSUpds (map (@xformSubstepRec _) ss)).
+    pose proof (wellHiddenSpec o HWellHidden) as sth.
+    pose proof (StepIntro (substepsSpecComb ssGd)) as final.
+    rewrite xformLabelHide in *.
+    specialize (final sth); clear sth.
+    constructor.
+    - intuition.
+    - apply unionCommute; intuition.
+    - intuition.
+  Qed.
+
+  Lemma rleEmpty m o u cs:
+    Substep m o u (Rle None) cs -> u = M.empty _ /\ cs = M.empty _.
+  Proof.
+    clear;
+    intros.
+    inversion H; intuition.
+  Qed.
+
+  Lemma methEmpty m o u cs:
+    Substep m o u (Meth None) cs -> u = M.empty _ /\ cs = M.empty _.
+  Proof.
+    clear;
+    intros.
+    inversion H; intuition.
+  Qed.
+
+  Theorem decomposition':
+    forall s sig, Behavior imp s sig ->
+                  exists sigSpec, Behavior spec (theta s) sigSpec /\
+                                  equivalentLabelSeq (mapSet p) sig sigSpec.
+  Proof.
+    intros.
+    dependent induction H.
+    dependent induction HMultistepBeh; subst.
+    - exists nil; rewrite thetaInit; repeat constructor.
+    - specialize (IHHMultistepBeh specCanCombine substepMethMap substepRuleMap
+                                  callSubset defSubset thetaGood thetaInit eq_refl).
+      clear defSubset0 callSubset0 thetaInit0 thetaGood0
+            substepRuleMap0 substepMethMap0 specCanCombine0.
+      pose proof (stepMap HStep) as [uSpec [stepSpec upd]].
+      destruct IHHMultistepBeh as [sigSpec [behSpec eqv]].
+      inversion behSpec; subst.
+      pose proof (BehaviorIntro (Multi HMultistepBeh0 stepSpec)) as sth.
+      rewrite upd in sth.
+      exists (xformLabel n l :: sigSpec).
+      constructor.
+      + intuition.
+      + constructor.
+        * unfold equivalentLabel, xformLabel; simpl.
+          destruct l; destruct annot; simpl; intuition.
+          destruct o; simpl; intuition.
+        * intuition.
+  Qed.
+
+  Theorem decomposition:
+    traceRefines (mapSet p) imp spec.
+  Proof.
+    unfold traceRefines; intros.
+    pose proof (decomposition' H) as [sigSpec beh].
+    exists (theta s1); exists sigSpec.
+    intuition.
+  Qed.
+End Decomposition.
