src/SemanticsOld.v
@@ -1,0 +1,445 @@
+Require Import Lib.CommonTactics Lib.FMap Lib.Struct.
+Require Export Syntax SemanticsExprAction. (* Should be "Require Export" *)
+Require Import String List.
+
+Set Implicit Arguments.
+
+Record LabelTP {A : Type} :=
+  { ruleMeth : option A
+  ; dms : CallsT
+  ; cms : CallsT
+  }.
+
+Arguments LabelTP : clear implicits.
+
+Definition LabelT := LabelTP True.
+Definition RuleLabelT := LabelTP string.
+
+Definition mapLabelTP {A B : Type} (f : A -> B) (l : LabelTP A)
+: LabelTP B :=
+  match l with
+    | Build_LabelTP rm dms cms => Build_LabelTP (option_map f rm) dms cms
+  end.
+
+Definition NotBothRule (rm1 rm2 : option string) : Prop :=
+  rm1 = None \/ rm2 = None.
+
+Definition CanCombine (ul1 ul2: RegsT * RuleLabelT) : Prop :=
+  M.Disj (fst ul1) (fst ul2) /\
+  NotBothRule (ruleMeth (snd ul1)) (ruleMeth (snd ul2)) /\
+  M.Disj (dms (snd ul1)) (dms (snd ul2)) /\
+  M.Disj (cms (snd ul1)) (cms (snd ul2)).
+
+Definition mergeLabel {A : Type} (l1 l2 : LabelTP A) : LabelTP A := 
+  match l1, l2 with
+      Build_LabelTP rm1 ds1 cs1, Build_LabelTP rm2 ds2 cs2 =>
+      Build_LabelTP (match rm1 with | Some r => Some r | None => rm2 end) 
+                    (M.union ds1 ds2) 
+                    (M.union cs1 cs2)
+  end.
+
+Definition equivalent {A : Type} (l1 l2 : LabelTP A)
+           (p : LabelTP A -> LabelTP A) :=
+  l1 = p l2.
+
+Local Open Scope string.
+
+Inductive UnitStep : Modules -> RegsT -> RegsT -> RuleLabelT -> Type :=
+| EmptyStep :
+    forall (regInits : list RegInitT)
+           (rules : list (Attribute (Action Void)))
+           (meths : list DefMethT)
+           (oRegs : RegsT),
+      M.KeysSubset oRegs (namesOf regInits) ->
+      UnitStep (Mod regInits rules meths) oRegs (M.empty _)
+               (Build_LabelTP None (M.empty _) (M.empty _))
+| SingleRule : 
+  forall (ruleName : string) (ruleBody : Action (Bit 0))
+         (regInits : list RegInitT)
+         (rules : list (Attribute (Action Void)))
+         (meths : list DefMethT),
+    In (ruleName :: ruleBody)%struct rules ->
+    forall (oRegs news : RegsT) (calls : CallsT)
+           (retV : type (Bit 0)),
+      SemAction oRegs (ruleBody type) news calls retV ->
+      M.KeysSubset oRegs (namesOf regInits) ->
+      UnitStep (Mod regInits rules meths) oRegs news
+               (Build_LabelTP (Some ruleName) (M.empty _) calls)
+| SingleMeth :
+    forall (regInits : list RegInitT)
+           (rules : list (Attribute (Action Void)))
+           (meths : list DefMethT)
+           (oRegs : RegsT)
+           (calls : CallsT) (news : RegsT) 
+           (meth : DefMethT),
+      In meth meths ->
+      forall (argV : type (arg (objType (attrType meth))))
+             (retV : type (ret (objType (attrType meth))))
+             (udefs : CallsT),
+        SemAction oRegs (objVal (attrType meth) type argV) news calls retV ->
+        udefs = M.add meth {|
+                        objType := objType (attrType meth);
+                        objVal := (argV, retV) |} (M.empty _) ->
+        M.KeysSubset oRegs (namesOf regInits) ->
+        UnitStep (Mod regInits rules meths) oRegs news
+                 (Build_LabelTP None udefs calls)
+| LeftIntro :
+    forall (m1 m2 : Modules)
+           (oRegs1 oRegs2 oRegs news : RegsT)
+           (l : RuleLabelT),
+      M.KeysSubset oRegs2 (namesOf (getRegInits m2)) ->
+      UnitStep m1 oRegs1 news l ->
+      oRegs = M.union oRegs1 oRegs2 ->
+      UnitStep (ConcatMod m1 m2) oRegs news l
+| RightIntro :
+    forall (m1 m2 : Modules)
+           (oRegs1 oRegs2 oRegs news : RegsT)
+           (l : RuleLabelT),
+      M.KeysSubset oRegs1 (namesOf (getRegInits m1)) ->
+      UnitStep m2 oRegs2 news l ->
+      oRegs = M.union oRegs1 oRegs2 ->
+      UnitStep (ConcatMod m1 m2) oRegs news l.
+
+Inductive UnitSteps (m : Modules) (o : RegsT) : RegsT -> RuleLabelT -> Type :=
+| UnitSteps1 : forall {u l}, UnitStep m o u l -> UnitSteps m o u l
+| UnitStepsUnion : forall {u1 u2 : RegsT} {l1 l2 : RuleLabelT}, 
+                     UnitSteps m o u1 l1 -> UnitSteps m o u2 l2 
+                     -> CanCombine (u1, l1) (u2, l2)
+                     -> UnitSteps m o (M.union u1 u2) (mergeLabel l1 l2).
+
+Definition signIsEq :
+  forall (l1 l2 : Typed SignT), sumbool (l1 = l2) (l1 <> l2).
+Proof.
+  intros. destruct l1, l2. 
+  destruct (SignatureT_dec objType objType0).
+  - induction e. destruct objType, objVal, objVal0.
+    destruct (isEq arg t t1). induction e.
+    destruct (isEq ret t0 t2). induction e. left. reflexivity.
+    right. unfold not. intros. apply typed_eq in H.
+    inversion H. apply n in H1. assumption.
+    right. unfold not. intros. apply typed_eq in H.
+    inversion H. apply n in H1. assumption.
+  - right. unfold not. intros. inversion H. apply n in H1.
+    assumption.
+Qed.
+
+Definition hide {A : Type} (l : LabelTP A) : LabelTP A :=
+  match l with
+      Build_LabelTP rm ds cs => 
+      Build_LabelTP rm (M.subtractKV signIsEq ds cs)
+                    (M.subtractKV signIsEq cs ds)
+  end.
+
+Definition wellHidden {A : Type} (l : LabelTP A) (m : Modules) :=
+  match l with
+      Build_LabelTP rm ds cs =>
+      M.KeysDisj ds (getCmsMod m)
+      /\ M.KeysDisj cs (getDmsMod m)
+  end.
+
+Inductive Step (m : Modules) (o u : RegsT) : RuleLabelT -> Type :=
+  MkStep : forall {l l': RuleLabelT},
+             UnitSteps m o u l ->
+             l' = hide l -> wellHidden l' m ->
+             Step m o u l'.
+
+Inductive MultiStep (m : Modules) (regs : RegsT) : RegsT -> list RuleLabelT -> Prop :=
+| MSNil : MultiStep m regs regs nil
+| MSMulti :
+    forall regs' labels,
+      MultiStep m regs regs' labels ->
+      forall l u,
+        Step m regs' u l ->
+        forall (regs'' : RegsT),
+          regs'' = M.update regs' u ->
+          MultiStep m regs regs'' (l :: labels).
+
+Section MakeMap.
+  Variable A: Type.
+  Variable f1 f2: A -> Type.
+  Variable f: forall x, f1 x -> f2 x.
+
+  Fixpoint makeMap (l: list (Attribute (Typed f1))) : M.t (Typed f2) :=
+    match l with
+      | nil => M.empty _
+      | {| attrName := n; attrType := {| objVal := rv |} |} :: xs =>
+        M.add n {| objVal := f rv |} (makeMap xs)
+    end.  
+End MakeMap.
+
+Definition initRegs (init: list RegInitT): RegsT := makeMap (fullType type) evalConstFullT init.
+Hint Unfold initRegs.
+
+Inductive Behavior (m : Modules) : RegsT -> list LabelT -> Prop :=
+  MkBehavior :
+    forall newRegs labels labels',
+      MultiStep m (initRegs (getRegInits m)) newRegs labels ->
+      labels' = (List.map (mapLabelTP (fun _ => I)) labels) ->
+      Behavior m newRegs labels'.
+
+Definition TraceRefines (mimpl mspec : Modules) (f : LabelT -> LabelT) :=
+  forall simp limp,        Behavior mimpl simp         limp ->
+  exists (sspec : RegsT),  Behavior mspec sspec (map f limp).
+
+Section Decomposition.
+  Variable rulesImp rulesSpec: list string.
+  Variable dmsImp dmsSpec: list DefMethT.
+  Variable imp spec: Modules.
+  Variable stateMap: RegsT -> RegsT.
+  Variable ruleMap: string -> string.
+  Variable p : (CallsT * CallsT) -> (CallsT * CallsT).
+
+  Definition pMod {A : Type} (f : A -> A) (l : LabelTP A) : LabelTP A
+    := match l with
+    | Build_LabelTP rm dm cm => let (dm', cm') := p (dm, cm) in
+       Build_LabelTP (option_map f rm) dm' cm'
+    end.
+
+  Definition pRL := pMod ruleMap.
+
+  Hypothesis pmerge : forall (ds1 ds2 cs1 cs2 : CallsT) (rm1 rm2 : option string)
+    , let l1 := Build_LabelTP rm1 ds1 cs1 in 
+      let l2 := Build_LabelTP rm2 ds2 cs2 in
+       M.Disj ds1 ds2 -> M.Disj cs1 cs2
+     -> NotBothRule rm1 rm2
+     -> mergeLabel (pRL l1) (pRL l2) = pRL (mergeLabel l1 l2).
+
+  Hypothesis phide : forall (l : RuleLabelT), pRL (hide l) = hide (pRL l).
+
+  Hypothesis pwellHidden : forall (l : RuleLabelT), 
+   wellHidden (hide l) imp -> wellHidden (pRL (hide l)) spec.
+
+  Variable T : forall {oImp nImp lImp}, UnitStep imp oImp nImp lImp 
+             -> (RegsT * RuleLabelT).
+
+  Fixpoint Ts {oImp nImp lImp} (steps : UnitSteps imp oImp nImp lImp)
+      : RegsT * RuleLabelT
+      := match steps with
+    | UnitSteps1 _ _ step => T step
+    | UnitStepsUnion _ _ _ _ step1 step2 canCombine => 
+      let (u1, l1) := Ts step1 in
+      let (u2, l2) := Ts step2 in
+      (M.union u1 u2, mergeLabel l1 l2)
+    end.
+
+  Let Ts' {oImp nImp lImp} (step : Step imp oImp nImp lImp)
+      : RegsT * RuleLabelT
+      := match step with
+    | MkStep _ _ steps _ _  => Ts steps
+    end.
+
+  Hypothesis stateMapBeginsWell :
+    stateMap (initRegs (getRegInits imp)) = initRegs (getRegInits spec).
+
+  Hypothesis stateMapModular : forall (oImp u1 u2 uSpec1 uSpec2 : RegsT),
+    M.Disj u1 u2 -> M.Disj uSpec1 uSpec2
+  -> M.update (stateMap oImp) uSpec1 = stateMap (M.update oImp u1)
+  -> M.update (stateMap oImp) uSpec2 = stateMap (M.update oImp u2)
+  -> M.update (stateMap oImp) (M.union uSpec1 uSpec2) 
+  = stateMap (M.update oImp (M.union u1 u2)).
+
+  Hypothesis consistentSubstepMap : forall {oImp lImp nImp}
+   , (exists ruleLabel, Behavior imp oImp ruleLabel)
+   -> forall (step : UnitStep imp oImp nImp lImp)
+   , match T step with (nSpec, lSpec) =>
+      let oSpec := stateMap oImp in
+        (M.update oSpec nSpec = stateMap (M.update oImp nImp)
+      /\ equivalent lSpec lImp pRL)
+      * UnitStep spec oSpec nSpec lSpec
+     end.
+
+  Hypothesis specShouldCombine : forall {oImp} 
+  , (exists ruleLabel, Behavior imp oImp ruleLabel)
+  -> forall {nImp1 lImp1} (step1 : UnitStep imp oImp nImp1 lImp1)
+      {nImp2 lImp2} (step2 : UnitStep imp oImp nImp2 lImp2)
+  , CanCombine (nImp1, lImp1) (nImp2, lImp2)
+  -> CanCombine (T step1) (T step2).
+
+  Lemma pBeforeAfter : forall (l : RuleLabelT),
+    pMod id (mapLabelTP (fun _ : string => I) l) =
+     mapLabelTP (fun _ : string => I) (pRL l).
+  Proof. intros. unfold pRL, pMod.
+  destruct l. simpl.
+  destruct (p (dms0, cms0)). simpl.
+  destruct ruleMeth0; simpl; unfold id; reflexivity.
+  Qed.
+
+  Lemma canCombineLeft :
+    forall {t u1 u2 l1 l2},
+      CanCombine t (M.union u1 u2, mergeLabel l1 l2) ->
+      CanCombine t (u1, l1).
+  Proof. 
+    intros.
+    destruct l1 as [rm1 ds1 cs1].
+    destruct l2 as [rm2 ds2 cs2].
+    unfold CanCombine in H; dest; simpl in *.
+    constructor; try (eapply M.Disj_union_1; eassumption).
+    unfold NotBothRule in *.
+    destruct rm1.
+    - simpl; destruct H0; [|discriminate].
+      repeat split.
+      + left; auto.
+      + eapply M.Disj_union_1; eauto.
+      + eapply M.Disj_union_1; eauto.
+    - repeat split.
+      + right; auto.
+      + eapply M.Disj_union_1; eauto.
+      + eapply M.Disj_union_1; eauto.
+  Qed.
+
+  Lemma canCombineRight :
+    forall {t u1 u2 l1 l2},
+      CanCombine t (M.union u1 u2, mergeLabel l1 l2) ->
+      CanCombine t (u2, l2).
+  Proof.
+    intros.
+    destruct l1 as [rm1 ds1 cs1].
+    destruct l2 as [rm2 ds2 cs2].
+    unfold CanCombine in H; dest; simpl in *.
+    constructor; try (eapply M.Disj_union_2; eassumption).
+    unfold NotBothRule in *.
+    destruct rm1.
+    - simpl; destruct H0; [|discriminate].
+      repeat split.
+      + left; auto.
+      + eapply M.Disj_union_2; eauto.
+      + eapply M.Disj_union_2; eauto.
+    - simpl; destruct H0.
+      + repeat split.
+        * left; auto.
+        * eapply M.Disj_union_2; eauto.
+        * eapply M.Disj_union_2; eauto.
+      + repeat split.
+        * right; auto.
+        * eapply M.Disj_union_2; eauto.
+        * eapply M.Disj_union_2; eauto.
+  Qed.
+
+  Lemma canCombineMerge : forall {t u1 u2 l1 l2},
+    CanCombine t (u1, l1)
+  -> CanCombine t (u2, l2)
+  -> CanCombine t (M.union u1 u2, mergeLabel l1 l2).
+  Proof.
+    admit.
+    (* intros. destruct t as [uL [rmL csL dsL]].  *)
+    (* destruct (mergeLabel l1 l2) as [rm1 cs ds] eqn:labeleqn. *)
+    (* inversion H; inversion H0; inversion labeleqn; subst. *)
+    (* econstructor. apply M.Disj_union; assumption. *)
+    (* apply M.Disj_union; assumption. *)
+    (* apply M.Disj_union; assumption. *)
+    (* unfold NotBothRule in *; destruct rmL, rm2, rm4; intuition. *)
+  Qed.  
+
+  Lemma canCombineSym : forall {t1 t2},
+    CanCombine t1 t2 -> CanCombine t2 t1.
+  Proof.
+    admit.
+   (* intros t1 t2 H; *)
+   (* inversion H; clear H; subst;  *)
+   (* constructor; eauto using M.Disj_comm. *)
+   (* unfold NotBothRule in *. *)
+   (* destruct rm1, rm2; intuition. *)
+  Qed. 
+
+  Lemma specShouldCombines : forall {oImp} 
+  , (exists ruleLabel, Behavior imp oImp ruleLabel)
+  -> forall {nImp1 lImp1} (step1 : UnitSteps imp oImp nImp1 lImp1)
+      {nImp2 lImp2} (step2 : UnitSteps imp oImp nImp2 lImp2)
+  , CanCombine (nImp1, lImp1) (nImp2, lImp2)
+  -> CanCombine (Ts step1) (Ts step2).
+  Proof. 
+    intros oImp H nImp1 lImp1 US1. induction US1.
+    - intros nImp2 lImp2 US2. induction US2.
+      + apply specShouldCombine; assumption.
+      + intros.
+        simpl in IHUS2_1, IHUS2_2.
+        pose proof (IHUS2_1 (canCombineLeft H0)) as H21.
+        pose proof (IHUS2_2 (canCombineRight H0)) as H22.
+        simpl. destruct (Ts US2_1). destruct (Ts US2_2).
+        apply canCombineMerge; assumption.
+    - simpl in *. intros. apply canCombineSym.
+      destruct (Ts US1_1). destruct (Ts US1_2).
+      apply canCombineMerge; apply canCombineSym;
+      [apply IHUS1_1 | apply IHUS1_2]; try assumption;
+      apply canCombineSym in H0;
+      apply canCombineSym. 
+      eapply canCombineLeft; eassumption.
+      eapply canCombineRight; eassumption.    
+  Qed.
+  
+Require CommonTactics.
+
+  Lemma consistentUnitStepsMap : forall oImp lImp nImp
+    , (exists ruleLabel, Behavior imp oImp ruleLabel)
+      -> forall (steps : UnitSteps imp oImp nImp lImp)
+      , let (nSpec, lSpec) := Ts steps in
+        let oSpec := stateMap oImp in
+        (M.update oSpec nSpec = stateMap (M.update oImp nImp)
+         /\ equivalent lSpec lImp pRL)
+        * UnitSteps spec oSpec nSpec lSpec.
+  Proof.
+    admit.
+  (*   intros. *)
+  (*   induction steps; intros. *)
+  (*   - pose proof (consistentSubstepMap H u0). simpl in *. *)
+  (*     destruct (T u0) as [uSpec lSpec]. *)
+  (*     intuition. constructor. assumption. *)
+  (* - pose proof (specShouldCombines H steps1 steps2 c). *)
+  (*   simpl in *. *)
+  (*   destruct (Ts steps1) as [uSpec1 lSpec1]. *)
+  (*   destruct (Ts steps2) as [uSpec2 lSpec2]. *)
+  (*   intuition.  *)
+  (*   CommonTactics.inv c. CommonTactics.inv H0. *)
+  (*   apply stateMapModular; assumption. *)
+  (*   unfold equivalent in *. subst. *)
+  (*   CommonTactics.inv c. *)
+  (*   apply pmerge; assumption. *)
+  (*   apply UnitStepsUnion. assumption. assumption. *)
+  (*   unfold equivalent in *. *)
+  (*   assumption. *)
+  Qed.
+  
+  Lemma consistentStepMap : forall oImp lImp nImp
+    , (exists ruleLabel, Behavior imp oImp ruleLabel)
+      -> forall (step : Step imp oImp nImp lImp)
+      , let (nSpec, lSpec) := Ts' step in
+        let oSpec := stateMap oImp in
+        (M.update oSpec nSpec = stateMap (M.update oImp nImp))
+        * Step spec oSpec nSpec (pRL lImp).
+  Proof. 
+    intros.
+    destruct step eqn:stepeqn.
+    pose proof (consistentUnitStepsMap H u). simpl in *.
+    destruct (Ts u) as [nSpec lSpec]. 
+    intuition.  
+    econstructor. eassumption.
+    unfold equivalent in *. rewrite e.
+    rewrite H1. apply phide.
+    unfold equivalent in *. subst.
+    apply (pwellHidden _ w).
+  Qed. 
+
+  Theorem decomposition : TraceRefines imp spec (pMod id).
+  Proof.
+    unfold TraceRefines. intros.
+    exists (stateMap simp).
+    pose proof H.
+    inversion H0; clear H0; subst.
+    econstructor.
+    Focus 2. instantiate (1 := map pRL labels).
+    repeat rewrite map_map. apply map_ext.
+    intros. apply pBeforeAfter.
+    induction H1.
+    - rewrite <- stateMapBeginsWell. apply MSNil.
+    - assert (Behavior imp regs' (map (mapLabelTP (fun _ : string => I)) labels)).
+      econstructor. eassumption. reflexivity.
+      pose proof (consistentStepMap (ex_intro _ _ H2) X).
+      destruct (Ts' X) eqn:Ts'X.
+      destruct X0 as [HT1 HT2].
+      apply MSMulti with (regs' := stateMap regs') (u := r).
+      apply IHMultiStep. assumption.
+      assumption.
+      rewrite H0. rewrite <- HT1. reflexivity.
+  Qed.
+
+End Decomposition.
